checker/theories/uGraph.v
@@ -751,7 +751,7 @@ Proof.
 Qed.
 
 
-Lemma make_graph_invariants uctx (Hi : global_gc_uctx_invariants uctx)
+Global Instance make_graph_invariants uctx (Hi : global_gc_uctx_invariants uctx)
   : invariants (make_graph uctx).
 Proof.
   split; [|split].
@@ -909,20 +909,16 @@ Section MakeGraph.
       apply make_graph_spec'. assumption.
   Defined.
 
-  Corollary consistent_no_loop : gc_consistent ctrs -> acyclic_no_loop G.
+  Global Instance consistent_no_loop : gc_consistent ctrs -> acyclic_no_loop G.
   Proof.
     intro. apply acyclic_caract1, make_graph_spec2.
     now apply make_graph_invariants. assumption.
   Defined.
 End MakeGraph.
 
-Existing Class invariants.
-Existing Instance make_graph_invariants.
-Existing Class acyclic_no_loop.
 Existing Class gc_consistent.
 Existing Class global_gc_uctx_invariants.
 Existing Class global_uctx_invariants.
-Existing Instance consistent_no_loop.
 Existing Instance gc_of_uctx_invariants.
 
 (** ** Check of consistency ** *)
